| Created  | Difficulty | Tags |
| -------- | ---------- | ---- |
| 2025-04-13 | Medium | 2d-array |



# [1143. Longest Common Subsequence](https://leetcode.com/problems/longest-common-subsequence)

Given two strings `text1` and `text2`, return the length of their longest **common subsequence** . If there is no **common subsequence** , return `0`.

A **subsequence**  of a string is a new string generated from the original string with some characters (can be none) deleted without changing the relative order of the remaining characters.

- For example, `"ace"` is a subsequence of `"abcde"`.

A **common subsequence**  of two strings is a subsequence that is common to both strings.

**Example 1:** 

```
Input: text1 = "abcde", text2 = "ace" 
Output: 3  
Explanation: The longest common subsequence is "ace" and its length is 3.
```

**Example 2:** 

```
Input: text1 = "abc", text2 = "abc"
Output: 3
Explanation: The longest common subsequence is "abc" and its length is 3.
```

**Example 3:** 

```
Input: text1 = "abc", text2 = "def"
Output: 0
Explanation: There is no such common subsequence, so the result is 0.
```

**Constraints:** 

- `1 <= text1.length, text2.length <= 1000`
- `text1` and `text2` consist of only lowercase English characters.

## Approach

- 2d-array dp, dp[i] [j] represents the longest common subsequence between substring `str1(0, i)` vs `str1(0, j)`, note here substring is of index [0, i - 1] and [0, j - 1].

  - If `str1.charAt(i) == str2.charAt(j)`, then dp[i] [j] = dp[i - 1] [j - 1] + 1;
  - If not equal, dp[i] [j] = max value between dp[i - 1] [j], dp[i] [j - 1]
  - Iterate from 0 to n
  - Initial case, dp[0] [j] = 0 and dp [i] [0] = 0

- 2d-array can be simplified into 1d-array to save space, with an additional value to store dp[i - 1] [j - 1]

  - dp[j] = prev + 1 when `str1.charAt(i) == str2.charAt(j)`, prev value is dp[j - 1] value before update.
  - dp[j] = max (dp[j], dp[j - 1]). Here dp[j - 1] is updated which is equivalent to dp[i] [j - 1], and dp[j] is not updated yet which is equivalent to dp[i - 1] [j]

  
## Solution

```java
// 2d array
public int longestCommonSubsequence(String text1, String text2) {
    int m = text1.length();
    int n = text2.length();
    int[][] dp = new int[m + 1][n + 1];
  
    for (int i = 1 ; i <= m ; i++) {
        for (int j = 1; j <= n; j++) {
            if (text1.charAt(i - 1) == text2.charAt(j - 1)) {
                dp[i][j] = dp[i - 1][j - 1] + 1;
            } else {
                dp[i][j] = Math.max(dp[i - 1][j], dp[i][j - 1]);
            }
        }
    }
    return dp[m][n];
}

// 1d-array
public int longestCommonSubsequence(String text1, String text2) {
    int m = text1.length();
    int n = text2.length();
    int[] dp = new int[n + 1];
 
  	int prev = 0;
    for (int i = 1 ; i <= m ; i++) {
      	prev = dp[0];
        for (int j = 1; j <= n; j++) {
          	// store dp[j] value (dp[i - 1][j]) before update it
          	int tmp = dp[j];
            if (text1.charAt(i - 1) == text2.charAt(j - 1)) {
              	// prev holds dp[i - 1][j - 1] value
                dp[j] = prev + 1;
            } else {
                dp[j] = Math.max(dp[j], [j - 1]);
            }
          	// update prev value
         		prev = tmp;
        }
    }
    return dp[n];
}
```

## Complexity Analysis

- Time complexity: O(M*N), in any case, the func will iterate 2 strings.
- Space complexity: O(M*N) for 2d-array, O(N) for 1d array. 

## Reflections

